fibration

ground_zero/HITs/interval.lean
@@ -132,32 +132,6 @@ namespace interval
 
   notation r `∧`:70 s := min r s
   notation r `∨`:70 s := max r s
-
-  inductive leg {α : Sort u} : α → Type u
-  | lam (f : I → α) : leg (f 0)
-
-  inductive post {α : Sort u} : α → Type u
-  | lam (f : I → α) : post (f 1)
-
-  def lifting_property {α : Sort u} {β : Sort v} (p : α → β) :=
-  Π {x : α}, leg (p x) → leg x
-
-  def fibration (α : Sort u) (β : Sort v) :=
-  Σ' (p : α → β), lifting_property p
-
-  notation α ` ↠ ` β := fibration α β
-
-  lemma lifting {α : Sort u} {β : α → Sort v} (f : I → α)
-    (u : β (f 0)) : @leg (psigma β) ⟨f 0, u⟩ :=
-  @leg.lam (psigma β) (λ i, ⟨f i,
-    @interval.ind (β ∘ f) u (types.equiv.subst seg u)
-      (types.equiv.path_over_subst types.eq.rfl) i⟩)
-
-  theorem type_family {α : Sort u} (β : α → Sort v) :
-    (Σ' x, β x) ↠ α := begin
-    existsi psigma.fst, intros x f,
-    cases x with x u, cases f with f u, apply lifting
-  end
 end interval
 
 end HITs
