ground_zero/theorems/fibration.lean
@@ -1,0 +1,53 @@
+import ground_zero.HITs.interval ground_zero.types.sigma
+open ground_zero ground_zero.HITs ground_zero.HITs.interval
+
+hott theory
+
+namespace ground_zero.theorems.fibration
+  universes u v
+
+  inductive leg {α : Sort u} : α → Type u
+  | lam (f : I → α) : leg (f 0)
+
+  inductive post {α : Sort u} : α → Type u
+  | lam (f : I → α) : post (f 1)
+
+  def lifting_property {α : Sort u} {β : Sort v} (p : α → β) :=
+  Π {x : α}, leg (p x) → leg x
+
+  def fibration (α : Sort u) (β : Sort v) :=
+  Σ' (p : α → β), lifting_property p
+
+  notation α ` ↠ ` β := fibration α β
+
+  lemma lifting {α : Sort u} {β : α → Sort v} (f : I → α)
+    (u : β (f 0)) : @leg (psigma β) ⟨f 0, u⟩ :=
+  @leg.lam (psigma β) (λ i, ⟨f i,
+    @interval.ind (β ∘ f) u (types.equiv.subst seg u)
+      (types.equiv.path_over_subst types.eq.rfl) i⟩)
+
+  theorem type_family {α : Sort u} (β : α → Sort v) :
+    (Σ' x, β x) ↠ α := begin
+    existsi psigma.fst, intros x f,
+    cases x with x u, cases f with f u, apply lifting
+  end
+
+  def forward {α : Sort u} {β : α → Sort v} (x : α) :
+    types.fib (@psigma.fst α β) x → β x
+  | ⟨⟨y, u⟩, h⟩ := types.equiv.subst h u
+
+  def backward {α : Sort u} {β : α → Sort v} (x : α) (u : β x) :
+    types.fib (@psigma.fst α β) x :=
+  ⟨⟨x, u⟩, by trivial⟩
+
+  theorem fiber_over {α : Sort u} {β : α → Sort v} (x : α) :
+    types.fib (@psigma.fst α β) x ≃ β x := begin
+    existsi (forward x), split; existsi (@backward α β x),
+    { intro u, cases u with u h, cases u with y u,
+      induction h, fapply types.sigma.prod,
+      { fapply types.sigma.prod; trivial },
+      { have p := types.sigma.prod_refl ⟨y, u⟩,
+        induction p, trivial } },
+    { intro u, trivial }
+  end
+end ground_zero.theorems.fibration
